testdata/wild/unused-import-aliased/unused-import-aliased.cue
@@ -1,0 +1,2 @@
+import m "math"
+x: 1
