testdata/wild/used-import-ok/used-import-ok.cue
@@ -1,0 +1,2 @@
+import "strings"
+x: strings.ToUpper("a")
